specs/experimental/rsapss/high-level/Spec.Bignum.Basic.fst
@@ -24,20 +24,17 @@ let bn_const_0 #n =
 let bn_cast_le #n m b = bn #m b
 let bn_cast_gt #n m b = bn #m b
 
+let bn_add #n #m a b =
+  assert (a + b < pow2 n);
+  let res = a + b in
+  bn #n res
+
 val lemma_bn_add:#n:size_pos -> #m:size_pos{n >= m} -> a:bignum n -> b:bignum m -> Lemma
   (bn_v a + bn_v b < pow2 (n + 1))
 let lemma_bn_add #n #m a b =
   pow2_le_compat n m;
   assert (bn_v a + bn_v b < pow2 n + pow2 n);
   pow2_double_sum n
-
-let bn_add #n #m a b =
-  lemma_bn_add #n #m a b;
-  assert (a + b < pow2 (n + 1));
-  let res = (a + b) % pow2 n in
-  let c = (a + b) / pow2 n in
-  lemma_div_lt (a + b) (n + 1) n;
-  (u8 c, bn #n res)
 
 let bn_add_carry #n #m a b =
   let res = a + b in
@@ -69,48 +66,15 @@ let bn_from_u64 c = bn #64 (uint_to_nat c)
 
 let bn_is_less #n #m x y = x < y
 
-val lemma_bn_lshift_mul_add:
-  #n:size_pos -> #m:size_pos -> x:bignum n -> i:size_nat -> y:bignum 64 -> z:bignum m -> Lemma
-  (requires (n + i + 64 <= m))
-  (ensures (bn_v x * pow2 i * bn_v y + bn_v z < pow2 (m + 1)))
-  #reset-options "--z3rlimit 30 --max_fuel 0"
-let lemma_bn_lshift_mul_add #n #m x i y z =
-  assert (bn_v x * pow2 i * bn_v y < pow2 n * pow2 i * pow2 64);
-  pow2_plus n i;
-  pow2_plus (n + i) 64;
-  assert (bn_v x * pow2 i * bn_v y + bn_v z < pow2 (n + i + 64) + pow2 m);
-  pow2_le_compat m (n + i + 64);
-  pow2_double_sum m
-
 let bn_lshift_mul_add #n #m x i y z =
-  lemma_bn_lshift_mul_add #n #m x i y z;
   let res = x * pow2 i * y + z in
-  assert (res < pow2 (m + 1));
-  let r = res % pow2 m in
-  let c = res / pow2 m in
-  lemma_div_lt res (m + 1) m;
-  (u8 c, bn #m r)
-
-val lemma_bn_lshift_add:
-  #n:size_pos -> #m:size_pos -> x:bignum n -> i:size_nat -> z:bignum m -> Lemma
-  (requires (n + i <= m))
-  (ensures (bn_v x * pow2 i + bn_v z < pow2 (m + 1)))
-  #reset-options "--z3rlimit 30 --max_fuel 0"
-let lemma_bn_lshift_add #n #m x i z =
-  assert (bn_v x * pow2 i < pow2 n * pow2 i);
-  pow2_plus n i;
-  assert (bn_v x * pow2 i+ bn_v z < pow2 (n + i) + pow2 m);
-  pow2_le_compat m (n + i);
-  pow2_double_sum m
+  assert (res < pow2 m);
+  bn #m res
 
 let bn_lshift_add #n #m x i z =
-  lemma_bn_lshift_add #n #m x i z;
   let res = x * pow2 i + z in
-  assert (res < pow2 (m + 1));
-  let r = res % pow2 m in
-  let c = res / pow2 m in
-  lemma_div_lt res (m + 1) m;
-  (u8 c, bn #m r)
+  assert (res < pow2 m);
+  bn #m res
 
 let bn_from_bytes_be #bBytes b =
   let res = nat_from_bytes_be b in
